\begin{mathpar}
  %%% Computation rules
  \inferrule*[Right=Ev-Term]
  { \texttt{assert($(\Gamma, \Delta), t$)} = \Gamma' }
  {(\Gamma, \Delta, t) \rightarrowtail (\Gamma', \Delta, \unit{}) }

  \inferrule*[Right=Ev-Sym]
  { \texttt{assert($(\Gamma, \Delta), s$)} = \Gamma'}
  { (\Gamma, \Delta, s) \rightarrowtail (\Gamma', \Delta, \unit{}) }
\end{mathpar}
% \inferrule*[Right=Ev-Chc]
%   { }
%   {(\Theta, \chc[D]{e_{1}, e_{2}}) \rightarrowtail (\Theta, \chc[D]{e_{1}, e_{2}})}
%
%   \hspace{0.5cm}
%   \inferrule*[Right=Ev-Unit]
%   { }
%   { (\Theta,\unit{}) \rightarrowtail (\Theta, \unit{}) }

  \begin{mathpar}
  %%%\unit{} elimination rules
  \inferrule*[Right=Ev-UL]
  {  }
  { (\Theta,\unit{} \wedge v) \rightarrowtail (\Theta, v) }

  \inferrule*[Right=Ev-UR]
  { }
  { (\Theta, v \wedge\unit{}) \rightarrowtail (\Theta, v)}
\end{mathpar}
\begin{mathpar}
%   \inferrule*[Right=Ev-DM-VOr]
%   { (\Theta ,\neg e_{1} \wedge \neg e_{2}) \rightarrowtail (\Theta', v)}
%   { (\Theta, \neg (e_{1} \vee e_{2})) \rightarrowtail (\Theta', v)}
%
%   \hspace{1cm}
%   \inferrule*[Right=Ev-DM-VAnd]
%   { (\Theta, \neg e_{1} \vee \neg e_{2}) \rightarrowtail (\Theta', v)}
%   { (\Theta, \neg (e_{1} \wedge e_{2})) \rightarrowtail (\Theta', v)}
%
  %%% Negation rules
  % \inferrule*[Right=Ev-NegS]
  % { (\Delta, \neg s) \mapsto (\Delta', s') \\
  %   ((\Gamma, \Delta'), s') \rightarrowtail (\Theta, \unit{})
  % }
  % { ((\Gamma, \Delta), \neg s) \rightarrowtail (\Theta, \unit{})}
%   \inferrule*[Right=Ev-Neg-Chc]
%   { }
%   { (\Theta, \neg \chc[D]{e_{1},e_{2}}) \rightarrowtail (\Theta, \chc[D]{\neg e_{1}, \neg e_{2}}) }
%
  \inferrule*[Right=Ev-Neg]
  { (\Delta,\neg v) \mapsto (\Delta', v')
    % ((\Gamma, \Delta') ,\neg v) \rightarrowtail (\Theta, v')
  }
  { (\Gamma, \Delta, \neg v) \rightarrowtail (\Gamma, \Delta', v') }
\end{mathpar}
  %%% And with Choice rules
% \begin{mathpar}
%   \hspace{-1.5cm}
%   \inferrule*[Right=Ev-And-ChcL]
%   { \Gamma, \Delta,e \rightarrowtail \Gamma', \Delta',e'}
%   { \Gamma, \Delta,\chc[D]{e_{1},e_{2}} \wedge e \rightarrowtail \Gamma',
%     \Delta',\chc[D]{e_{1},e_{2}} \wedge e' }
% \end{mathpar}
% \begin{mathpar}
%   \hspace{-1.5cm}
%   \inferrule*[Right=Ev-And-ChcR]
%   { \Gamma, \Delta,e \rightarrowtail \Gamma', \Delta',e'}
%   { \Gamma, \Delta,e \wedge \chc[D]{e_{1},e_{2}} \rightarrowtail \Gamma',
%     \Delta',e' \wedge \chc[D]{e_{1},e_{2}} }
%   % {l \rightarrowtail l'}
%   % { l \wedge \chc[D]{e_{1},e_{2}} \rightarrowtail l' \wedge \chc[D]{e_{1},e_{2}}}
% \end{mathpar}
%   %%% Or with Choice rules
% \begin{mathpar}
%   \hspace{-1.5cm}
%   \inferrule*[Right=Ev-Or-ChcL]
%   {\Delta,e \mapsto \Delta',v}
%   { \Gamma, \Delta,\chc[D]{e_{1},e_{2}} \vee e \rightarrowtail \Gamma,
%     \Delta',\chc[D]{e_{1},e_{2}} \vee v}
% \end{mathpar}
% \begin{mathpar}
%   \hspace{-1.5cm}
%   \inferrule*[Right=Ev-Or-ChcR]
%   {\Delta,e \mapsto \Delta',v}
%   { \Gamma, \Delta,e \vee \chc[D]{e_{1},e_{2}} \rightarrowtail \Gamma,
%     \Delta',v \vee \chc[D]{e_{1},e_{2}} }
% \end{mathpar}
% \begin{mathpar% }
%   \inferrule*[Right=Ev-Or-Value]
%   {(\Delta, e_{1}) \mapsto (\Delta_{1}, s_{1}) \\
%     (\Delta_{1}, e_{2}) \mapsto (\Delta_{2}, s_{2}) \\
%     (\Delta_{2}, s_{1} \vee s_{2}) \mapsto (\Delta_{s}, s) \\
%     ((\Gamma, \Delta_{s}), s) \twoheadrightarrow (\Theta,\unit{})
%   }
%   { ((\Gamma, \Delta),e_{1} \vee e_{2}) \rightarrowtail (\Theta,\unit{})}
% \end{mathpar}
  %%% Congruence rules with symbolic execution
\begin{mathpar}
  \inferrule*[Right=Ev-Or]
  { (\Delta, v_{1}) \mapsto (\Delta', v_{1}') \\
    (\Delta',v_{2}) \mapsto (\Delta'', v_{2}')}
  { (\Gamma, \Delta, v_{1} \vee v_{2}) \rightarrowtail (\Gamma, \Delta'', v_{1}' \vee v_{2}')}
\end{mathpar}%
\begin{mathpar}
  \inferrule*[Right=Ev-And]
  {(\Theta, v_{1}) \rightarrowtail (\Theta', v_{1}') \\
    (\Theta', v_{2}) \rightarrowtail (\Theta'', v_{2}')
  }
  { (\Theta, v_{1} \wedge v_{2}) \rightarrowtail (\Theta'', v_{1}' \wedge v_{2}')
  }
\end{mathpar}%
