\begin{mathpar}
\inferrule*[right=\acRef]
  { \pwrap{\pspawn}(\aStore{},r) = (\aStore{}', s) }
  { (\aStore{}, r) \accumulation (\aStore{}', s) }

\inferrule*[right=\acNotS]
  { (\aStore{}, v) \accumulation (\aStore{}', s) \\
    \pwrap{\pnot}(\aStore{}', s) = (\aStore{}'', s') }
  { (\aStore{}, \neg{} v) \accumulation (\aStore{}'', s') }

\inferrule*[right=\acAndS]
  { (\aStore{}, v_1) \accumulation (\aStore{1}, s_1) \\
    (\aStore{1}, v_2) \accumulation (\aStore{2}, s_2) \\
    \pwrap{\pand}(\aStore{2}, s_1, s_2) = (\aStore{3}, s_3) }
  { (\aStore{}, v_1 \wedge v_2) \accumulation{} (\aStore{3}, s_3) }

\inferrule*[right=\acOrS]
  { (\aStore{}, v_1) \accumulation (\aStore{1}, s_1) \\
    (\aStore{1}, v_2) \accumulation (\aStore{2}, s_2) \\
    \pwrap{\por}(\aStore{2}, s_1, s_2) = (\aStore{3}, s_3) }
  { (\aStore{}, v_1 \vee v_2) \accumulation{} (\aStore{3}, s_3) }

\inferrule*[right=\acChc]
  { }
  {(\aStore,\chc[D]{e_1,e_2}) \accumulation (\aStore{},\chc[D]{e_1,e_2})}

\inferrule*[right=\acNotV]
  { (\aStore{}, v) \accumulation (\aStore{}', v') }
  { (\aStore{}, \neg{} v) \accumulation (\aStore{}', \neg v') }

\inferrule*[right=\acAndV]
  { (\aStore{}, v_1) \accumulation (\aStore{1}, v_1') \\
    (\aStore{1}, v_2) \accumulation (\aStore{2}, v_2') }
  { (\aStore{}, v_1 \wedge v_2) \accumulation{} (\aStore{2}, v_1' \wedge v_2') }

\inferrule*[right=\acOrV]
  { (\aStore{}, v_1) \accumulation (\aStore{1}, v_1') \\
    (\aStore{1}, v_2) \accumulation (\aStore{2}, v_2') }
  { (\aStore{}, v_1 \vee v_2) \accumulation{} (\aStore{2}, v_1' \vee v_2') }
\end{mathpar}
