\begin{mathpar}
  %%% Computation rules
  \inferrule*[Right=Ac-Gen]
  { r \notin \kf{dom}(\Delta) \\
    \texttt{spawn($\Delta, r$)} = (\Delta', s)}
  {(\Delta, r) \mapsto (\Delta', s)}

  \inferrule*[Right=Ac-Ref]
  { \Delta(r) = s}
  {(\Delta, r) \mapsto (\Delta, s)}
  \\
  %%% Negation rules
  \inferrule*[Right=Ac-Neg]
  { \texttt{negate($\Delta, s$)} = (\Delta', s')}
  { (\Delta, \neg s) \mapsto (\Delta', s')}
\\
%   \hspace{0.7cm}
%   \inferrule*[Right=Ac-C]
%   { }
%   {(\Delta, \chc[D]{e_{1}, e_{2}}) \mapsto (\Delta, \chc[D]{e_{1}, e_{2}})}
%
% \begin{mathpar}
%   \inferrule*[Right=Ac-Neg-C]
%   { }
%   { (\Delta, \neg \chc[D]{e_{1},e_{2}}) \mapsto (\Delta, \chc[D]{\neg e_{1}, \neg e_{2}}) }
% % \end{mathpar}
%   \hspace{0.9cm}
%
% % \begin{mathpar}
%   \inferrule*[Right=Ac-Unit]
%   { }
%   { (\Delta, \bullet) \mapsto (\Delta, \unit{})}
% \end{mathpar}
%
  \inferrule*[Right=Ac-SOr]
  { \texttt{or($\Delta, s_{1}, s_{2}$)} = (\Delta', s') }
  {(\Delta, s_{1} \vee s_{2}) \mapsto (\Delta', s')}

  \inferrule*[Right=Ac-SAnd]
  { \texttt{and($\Delta, s_{1}, s_{2}$)} = (\Delta', s') }
  {(\Delta, s_{1} \wedge s_{2}) \mapsto (\Delta', s')}
\\
%
% \begin{mathpar}
%   \hspace{-1.5cm}
%   \inferrule*[Right=Ac-DM-VOr]
%   { }
%   { (\Delta, \neg (e_{1} \vee e_{2})) \mapsto (\Delta, \neg e_{1} \wedge
%     \neg e_{2}) }
% \end{mathpar}
%
% \begin{mathpar}
%   \hspace{-1.5cm}
%   \inferrule*[Right=Ac-DM-VAnd]
%   { }
%   { (\Delta, \neg (e_{1} \wedge e_{2})) \mapsto (\Delta, \neg e_{1}
%     \vee \neg e_{2}) }
% \end{mathpar}
%
%%% And with Choice rules
% \begin{mathpar}
%   \hspace{-1.5cm}
%   \inferrule*[Right=Ac-VAnd-ChcL]
%   {\Delta, e \mapsto \Delta', s}
%   { \Delta, \chc[D]{e_{1},e_{2}} \wedge e \mapsto \Delta', \chc[D]{e_{1},e_{2}} \wedge s}
% \end{mathpar}
%
% \begin{mathpar}
%   \hspace{-1.5cm}
%   \inferrule*[Right=Ac-VAnd-ChcR]
%   {\Delta, e \mapsto \Delta', s}
%   { \Delta, e \wedge \chc[D]{e_{1},e_{2}} \mapsto \Delta', s \wedge \chc[D]{e_{1},e_{2}} }
% \end{mathpar}
%
  %%% Or with Choice rules
% \begin{mathpar}
%   \hspace{-1.5cm}
%   \inferrule*[Right=Ac-VOr-ChcL]
%   {\Delta, e \mapsto \Delta', s}
%   { \Delta, \chc[D]{e_{1},e_{2}} \vee e \mapsto \Delta' \,
%     \chc[D]{e_{1},e_{2}} \vee s}
% \end{mathpar}
%
% \begin{mathpar}
%   \hspace{-1.5cm}
%   \inferrule*[Right=Ac-VOr-ChcR]
%   {\Delta, e \mapsto \Delta', s}
%   { \Delta, e \vee \chc[D]{e_{1},e_{2}} \mapsto \Delta', s \vee \chc[D]{e_{1},e_{2}} }
% \end{mathpar}
%
%%% Congruence rules with symbolic execution
% \end{mathpar}
%
% \begin{mathpar}
%   \hspace{-1.5cm}
%   \inferrule*[Right=Ac-VOr-Value]
%   {(\Delta, e_{1}) \mapsto (\Delta_{1}, s_{1}) \\ (\Delta_{1}, e_{2}) \mapsto
%     (\Delta_{2}, s_{2}) \\  (\Delta_{2}, s_{1} \vee s_{2}) \leadsto
%     (\Delta', s)}
%   { (\Delta, e_{1} \vee e_{2}) \mapsto (\Delta', s)}
% \end{mathpar}
%
% \begin{mathpar}
%   %%% Congruence rules with symbolic execution
%   \inferrule*[Right=Ac-VAnd]
%   {(\Delta, v_{1}) \mapsto (\Delta_{1}, v_{1}) \\ (\Delta_{1}, v_{2}) \mapsto
%     (\Delta', v_{2})}
%   {(\Delta, v_{1} \wedge v_{2}) \mapsto (\Delta', v_{1} \wedge v_{2})}
%
%   \inferrule*[Right=Ac-VOr]
%   {(\Delta, v_{1}) \mapsto (\Delta_{1}, v_{1}) \\
%     (\Delta_{1}, v_{2}) \mapsto (\Delta', v_{2})}
%   {(\Delta, v_{1} \vee v_{2}) \mapsto (\Delta', v_{1} \vee v_{2})}
% \end{mathpar}%
%
\end{mathpar}
%
% \begin{mathpar}
% \inferrule*[Right=Ac-And]
% {(\Delta, v_{1}) \mapsto (\Delta_{1}, v_{1}') \\ (\Delta_{1}, v_{2}) \mapsto (\Delta_{2}, v_{2}')}
% % ---------------------------------------------------------------
% { (\Delta, v_{1} \wedge v_{2}) \mapsto (\Delta_{2}, v_{1}' \wedge v_{2}') }
% \end{mathpar}
% %
% \begin{mathpar}
% \inferrule*[Right=Ac-Or]
% {(\Delta, v_{1}) \mapsto (\Delta_{1}, v_{1}') \\ (\Delta_{1}, v_{2}) \mapsto (\Delta_{2}, v_{2}')}
% % ---------------------------------------------------------------
% { (\Delta, v_{1} \vee v_{2}) \mapsto (\Delta_{2}, v_{1}' \vee v_{2}') }

% \end{mathpar}
