\begin{mathpar}
\inferrule*[right=\acRef]
  { \pwrap{\pspawn}(\aStore{},r) = (\aStore{}', s) }
  { (\aStore{}, r) \accumulation (\aStore{}', s) }

  \inferrule*[right=\acRefi]
  { \pwrap{\pspawni}(\aStore{},r_{i}) = (\aStore{}', s) }
  { (\aStore{}, r_{i}) \accumulation (\aStore{}', s) }

\inferrule*[right=\acNotS]
  { (\aStore{}, v) \accumulation (\aStore{}', s) \\
    \pwrap{\pnot}(\aStore{}', s) = (\aStore{}'', s') }
  { (\aStore{}, \neg{} v) \accumulation (\aStore{}'', s') }

  \inferrule*[right=\acNegS]
  { (\aStore{}, v) \accumulation (\aStore{}', s) \\
    \pwrap{\pneg}(\aStore{}', s) = (\aStore{}'', s') }
  { (\aStore{}, - v) \accumulation (\aStore{}'', s') }

\inferrule*[right=\acBoolS]
 { \op \in \boolFuncs{} \\
  (\aStore{}, v_1) \accumulation (\aStore{1}, s_1) \\
    (\aStore{1}, v_2) \accumulation (\aStore{2}, s_2) \\
    \lookup{\op}{\boolFuncs{}} \coloneqq \pwrap{\op} \\
    \pwrap{\op}(\aStore{2}, s_1, s_2) = (\aStore{3}, s_3) }
  { (\aStore{}, v_1\; \op\; v_2) \accumulation{} (\aStore{3}, s_3) }

  \inferrule*[right=\acArithS]
  { \op \in \integerFuncs{} \\
    (\aStore{}, v_1) \accumulation (\aStore{1}, s_1) \\
    (\aStore{1}, v_2) \accumulation (\aStore{2}, s_2) \\
    \lookup{\op}{\integerFuncs{}} \coloneqq \pwrap{\op} \\
    \pwrap{\op}(\aStore{2}, s_1, s_2) = (\aStore{3}, s_3) }
  { (\aStore{}, v_1\; \op\; v_2) \accumulation{} (\aStore{3}, s_3) }

  \inferrule*[right=\acInEqS]
  { \op \in\ \inequalities{} \\
    (\aStore{}, v_1) \accumulation (\aStore{1}, s_1) \\
    (\aStore{1}, v_2) \accumulation (\aStore{2}, s_2) \\
    \lookup{\op}{\inequalities} \coloneqq \pwrap{\op} \\
    \pwrap{\op}(\aStore{2}, s_1, s_2) = (\aStore{3}, s_3) }
  { (\aStore{}, v_1\; \op\; v_2) \accumulation{} (\aStore{3}, s_3) }

\inferrule*[right=\acChc]
  { }
  {(\aStore,\chc[D]{e_1,e_2}) \accumulation (\aStore{},\chc[D]{e_1,e_2})}

\inferrule*[right=\acNotV]
  { (\aStore{}, v) \accumulation (\aStore{}', v') }
  { (\aStore{}, \neg{} v) \accumulation (\aStore{}', \neg v') }

\inferrule*[right=\acAndV]
  { (\aStore{}, v_1) \accumulation (\aStore{1}, v_1') \\
    (\aStore{1}, v_2) \accumulation (\aStore{2}, v_2') }
  { (\aStore{}, v_1 \wedge v_2) \accumulation{} (\aStore{2}, v_1' \wedge v_2') }

\inferrule*[right=\acOrV]
  { (\aStore{}, v_1) \accumulation (\aStore{1}, v_1') \\
    (\aStore{1}, v_2) \accumulation (\aStore{2}, v_2') }
  { (\aStore{}, v_1 \vee v_2) \accumulation{} (\aStore{2}, v_1' \vee v_2') }
\end{mathpar}


% \begin{mathpar}
%   %%% Computation rules
%   \inferrule*[Right=Ac-Gen]
%   { r \notin{} \kf{dom} (\aStore{}) \quad{}
%     \texttt{Spawn(\aStore{},$r$)} = (\aStore{}', s)}
%   {(\aStore{}, r) \mapsto{} (\aStore{}', s)}
% \\
%   \inferrule*[Right=Ac-Geni]
%   { r \notin{} \kf{dom} (\aStore{}) \quad{}
%     \texttt{Spawn(\aStore{},$r_{i}$)} = (\aStore{}', s)}
%   {(\aStore{}, r_{i}) \mapsto{} (\aStore{}', s)}
% \end{mathpar}
% \begin{mathpar}
% \inferrule*[Right=Ac-Ref]
%   {\aStore{}(r) = s}
%   {(\aStore{}, r) \accumulation{} (\aStore{}, s)}

%   \inferrule*[Right=Ac-Refi]
%   {\aStore{}(r_{i}) = s}
%   {(\aStore{}, r_{i}) \accumulation{} (\aStore{}, s)}
% \\
% % \inferrule*[Right=Ac-Tm]
% % {\aStore{}(t) = s}
% % {(\aStore{}, t) \accumulation{} (\aStore{}, s)}

% % \inferrule*[Right=Ac-Tmi]
% % {\aStore{}(t_{i}) = s}
% % {(\aStore{}, t_{i}) \accumulation{} (\aStore{}, s)}
% % \\
% \inferrule*[Right=Ac-Chc]
% { }
% {(\aStore, \chc[D]{e_{1},e_{2}}) \accumulation{} (\aStore{}, \chc[D]{e_{1},e_{2}})}
% \\
%   %%% Negation rules
%   \inferrule*[Right=Ac-BU]
%   { \mathtt{Not}(\aStore{}, s) = (\aStore{}', s')}
%   { (\aStore{}, \neg{} s) \accumulation{} (\aStore{}', s')}

%   \inferrule*[Right=Ac-IU]
%   { \ui{}(\aStore{}, s) = (\aStore{}', s')}
%   { (\aStore{}, \integerUnary{}s) \accumulation{} (\aStore{}', s')}
% \\
%   \inferrule*[Right=Ac-SBinB]
%   { \bbb(\aStore, s_{1}, s_{2}) = (\aStore{}', s') }
%   {(\aStore{}, s_{1} \boolFuncs{} s_{2}) \accumulation{} (\aStore{}', s')}
%   \\
%   \inferrule*[Right=Ac-SBinI]
%   { \bii(\aStore, s_{1}, s_{2}) = (\aStore{}', s') }
%   {(\aStore{}, s_{1} \integerFuncs{} s_{2}) \accumulation{} (\aStore{}', s')}
%   \\
%   \inferrule*[Right=Ac-SBinIB]
%   { \bib(\aStore, s_{1}, s_{2}) = (\aStore{}', s') }
%   {(\aStore{}, s_{1} \inequalities{} s_{2}) \accumulation{} (\aStore{}', s')}
% \\
%   \inferrule*[Right=Ac-BinB]
%   { (\aStore{}, v_{1}) \accumulation{} (\aStore{1}, s_{1}) \\
%     (\aStore{1}, v_{2}) \accumulation{} (\aStore{}', s_{2}) \\
%   }
%   {(\aStore{}, v_{1} \boolFuncs{} v_{2}) \accumulation{} (\aStore{}', s_{1}
%     \boolFuncs s_{2})}

%   \inferrule*[Right=Ac-BinI]
%   { (\aStore{}, v_{1}) \accumulation{} (\aStore{1}, s_{1}) \\
%     (\aStore{1}, v_{2}) \accumulation{} (\aStore{}', s_{2}) \\
%   }
%   {(\aStore{}, v_{1} \integerFuncs{} v_{2}) \accumulation{} (\aStore{}', s_{1}
%     \integerFuncs{} s_{2})}

%   \inferrule*[Right=Ac-BinIB]
%   { (\aStore{}, v_{1}) \accumulation{} (\aStore{1}, s_{1}) \\
%     (\aStore{1}, v_{2}) \accumulation{} (\aStore{}', s_{2}) \\
%   }
%   {(\aStore{}, v_{1} \inequalities{} v_{2}) \accumulation{} (\aStore{}', s_{1}
%     \inequalities{} s_{2})}
% \end{mathpar}
